SyBlocToObc/Correctness.v
@@ -1,0 +1,37 @@
+Require Import Velus.Common.
+Require Import Velus.Operators.
+Require Import Velus.Clocks.
+
+Require Import Velus.NLustre.NLExprSyntax.
+Require Import Velus.NLustre.Stream.
+Require Import Velus.NLustre.NLExprSemantics.
+Require Import Velus.SyBloc.SBSyntax.
+Require Import Velus.SyBloc.SBSemantics.
+
+Require Import Velus.Obc.ObcSyntax.
+Require Import Velus.Obc.ObcSemantics.
+
+Require Import Velus.SyBlocToObc.Translation.
+
+Require Import List.
+Import List.ListNotations.
+
+Open Scope positive.
+Open Scope list.
+
+Module Type CORRECTNESS
+       (Import Ids     : IDS)
+       (Import Op      : OPERATORS)
+       (Import OpAux   : OPERATORS_AUX       Op)
+       (Import Clks    : CLOCKS          Ids)
+       (Import ExprSyn : NLEXPRSYNTAX        Op)
+       (Import SynSB   : SBSYNTAX        Ids Op       Clks ExprSyn)
+       (Import Str     : STREAM              Op OpAux)
+       (Import ExprSem : NLEXPRSEMANTICS Ids Op OpAux Clks ExprSyn              Str)
+       (Import SemSB   : SBSEMANTICS     Ids Op OpAux Clks ExprSyn SynSB        Str ExprSem)
+       (Import SynObc  : OBCSYNTAX       Ids Op OpAux)
+       (Import SemObc  : OBCSEMANTICS    Ids Op OpAux                    SynObc)
+       (Import Trans   : TRANSLATION     Ids Op OpAux Clks ExprSyn SynSB SynObc).
+
+
+End CORRECTNESS.
